SystemFD/Metatheory/Uniqueness.lean
@@ -1,0 +1,224 @@
+
+import SystemFD.Term
+import SystemFD.Term.Definition
+import SystemFD.Judgment
+import SystemFD.Ctx
+
+theorem no_valid_head_variable_with_all :
+  ¬ ValidHeadVariable (∀[A]B) test
+:= by
+intro h; unfold ValidHeadVariable at h
+cases h; case _ x h =>
+cases h; case _ h1 h2 =>
+  simp at h1
+
+theorem no_valid_head_variable_with_arrow :
+  ¬ ValidHeadVariable (A -t> B) test
+:= by
+intro h; unfold ValidHeadVariable at h
+cases h; case _ x h =>
+cases h; case _ h1 h2 =>
+  simp at h1
+
+theorem uniqueness_prefix_match :
+  PrefixTypeMatch Γ U V A ->
+  PrefixTypeMatch Γ U V B ->
+  A = B
+:= by
+intro j1 j2
+induction V generalizing Γ U A B
+any_goals try (
+  case _ =>
+    cases j1; case _ j1 =>
+    cases j2; case _ j2 =>
+      rfl
+)
+case _ v t1 t2 ih1 ih2 =>
+  cases v
+  any_goals try (
+    case _ =>
+      cases j1; case _ j1 =>
+      cases j2; case _ j2 =>
+        rfl
+  )
+  case _ =>
+    cases j1
+    case _ j1 =>
+      exfalso
+      apply no_valid_head_variable_with_all j1
+    case _ j1 =>
+    cases j2
+    case _ j2 =>
+      exfalso
+      apply no_valid_head_variable_with_all j2
+    case _ j2 =>
+      replace ih2 := ih2 j1 j2
+      have lem : [P][S]A = [P][S]B := by rw [ih2]
+      simp at lem; apply lem
+  case _ =>
+    cases j1
+    case _ j1 =>
+      exfalso
+      apply no_valid_head_variable_with_arrow j1
+    case _ j1 =>
+    cases j2
+    case _ j2 =>
+      exfalso
+      apply no_valid_head_variable_with_arrow j2
+    case _ j2 =>
+      replace ih2 := ih2 j1 j2
+      have lem : [P][S]A = [P][S]B := by rw [ih2]
+      simp at lem; apply lem
+
+theorem uniqueness_of_types :
+  Γ ⊢ t : A -> Γ ⊢ t : B -> A = B
+:= by
+intro j1 j2
+induction t generalizing Γ A B
+case _ => cases j1
+case _ x =>
+  cases j1; case _ q1 q2 =>
+  cases j2; case _ r1 r2 =>
+    generalize fdef : Γ d@ x = f at *
+    unfold Frame.get_type at *
+    cases f <;> simp at *
+    all_goals (subst q2; subst r2; rfl)
+case _ => cases j1; cases j2; rfl
+case _ v t ih =>
+  cases v
+  case _ =>
+    cases j1; case _ K1 q1 q2 =>
+    cases j2; case _ K2 r1 r2 =>
+      rfl
+  case _ =>
+    cases j1; case _ A1 B1 q1 =>
+    cases j2; case _ A2 B2 q2 =>
+      replace ih := ih q1 q2
+      injection ih with _ e1 e2
+      subst e1; subst e2; rfl
+  case _ =>
+    cases j1; case _ K1 q1 q2 =>
+    cases j2; case _ K2 r1 r2 =>
+      replace ih := ih q2 r2
+      injection ih with _ e1 e2
+      injection e1 with _ v1 v2
+      injection e2 with _ u1 u2
+      subst v1; subst v2; subst u1; subst u2
+      rfl
+  case _ =>
+    cases j1; case _ q1 =>
+    cases j2; case _ q2 =>
+      replace ih := ih q1 q2
+      injection ih with _ e1 e2
+      injection e1 with _ u1 u2
+      injection e2 with _ v1 v2
+      subst u1; subst u2; subst v1; subst v2
+      rfl
+case _ v t1 t2 ih1 ih2 =>
+  cases v
+  case _ =>
+    cases j1; case _ q =>
+    cases j2; case _ r =>
+      rfl
+  case _ =>
+    cases j1; case _ q =>
+    cases j2; case _ r =>
+      replace ih1 := ih1 q r
+      injection ih1 with _ e1 e2
+  case _ =>
+    cases j1; case _ q1 q2 q3 =>
+    cases j2; case _ r1 r2 r3 =>
+      replace ih1 := ih1 q1 r1
+      injection ih1 with _ e1 e2; subst e1; subst e2
+      subst q3; subst r3; rfl
+  case _ =>
+    cases j1; case _ q1 q2 q3 =>
+    cases j2; case _ r1 r2 r3 =>
+      replace ih1 := ih1 q1 r1
+      injection ih1 with _ e1 e2; subst e1; subst e2
+      subst q3; subst r3; rfl
+  case _ =>
+    cases j1; case _ q =>
+    cases j2; case _ r =>
+      replace ih2 := ih2 q r
+      injection ih2 with _ e1 e2
+  case _ =>
+    cases j1; case _ q1 q2 =>
+    cases j2; case _ r1 r2 =>
+      replace ih1 := ih1 q1 r1
+      replace ih2 := ih2 q2 r2
+      injection ih1 with _ e1 e2; subst e1; subst e2
+      injection ih2 with _ e1 e2; subst e2
+      rfl
+  case _ =>
+    cases j1; case _ q1 q2 =>
+    cases j2; case _ r1 r2 =>
+      replace ih1 := ih1 q1 r1
+      replace ih2 := ih2 q2 r2
+      injection ih1 with _ e1 e2; subst e1; subst e2
+      injection ih2 with _ e1 e2; subst e1; subst e2
+      rfl
+  case _ =>
+    cases j1; case _ q1 q2 =>
+    cases j2; case _ r1 r2 =>
+      replace ih1 := ih1 q1 r1
+      replace ih2 := ih2 q2 r2
+      injection ih1 with _ e1 e2;
+      injection e1 with _ w1 w2; subst w1; subst w2
+      injection e2 with _ _ w1; subst w1
+      injection ih2 with _ e1 e2; subst e1; subst e2
+      rfl
+  case _ =>
+    cases j1; case _ q =>
+    cases j2; case _ r =>
+      rfl
+case _ v t1 t2 ih1 ih2 =>
+  cases v
+  case _ =>
+    cases j1; case _ q1 =>
+    cases j2; case _ q2 =>
+      rfl
+  case _ =>
+    cases j1; case _ q1 =>
+    cases j2; case _ q2 =>
+      replace ih2 := ih2 q1 q2; subst ih2
+      rfl
+  case _ =>
+    cases j1; case _ q1 =>
+    cases j2; case _ q2 =>
+      replace ih2 := ih2 q1 q2; subst ih2
+      rfl
+  case _ =>
+    cases j1; case _ q1 =>
+    cases j2; case _ q2 =>
+      rfl
+  case _ =>
+    cases j1; case _ q1 =>
+    cases j2; case _ q2 =>
+      replace ih2 := ih2 q1 q2
+      injection ih2 with _ e1 e2
+      subst e1; subst e2; rfl
+  case _ =>
+    cases j1; case _ q1 q2 q3 =>
+    cases j2; case _ r1 r2 r3 =>
+      replace ih1 := ih1 q2 r2
+      replace ih2 := ih2 q3 r3
+      injection ih1 with _ e1 e2; subst e1; subst e2
+      injection ih2 with _ e1 e2; subst e1; subst e2
+      rfl
+case _ ih1 ih2 ih3 ih4 =>
+  cases j1; case _ q1 =>
+  cases j2; case _ r1 =>
+    replace ih4 := ih4 q1 r1; subst ih4; rfl
+case _ ih1 ih2 ih3 =>
+  cases j1; case _ q1 q2 q3 q4 q5 q6 =>
+  cases j2; case _ r1 r2 r3 r4 r5 r6 =>
+    replace ih1 := ih1 q1 r1; subst ih1
+    replace ih3 := ih3 q4 r4; subst ih3
+    apply uniqueness_prefix_match q5 r5
+case _ ih1 ih2 =>
+  cases j1; case _ q1 =>
+  cases j2; case _ r1 =>
+    replace ih2 := ih2 q1 r1;
+    have lem : [P][S]A = [P][S]B := by rw [ih2]
+    simp at lem; apply lem
