SystemFD/Term/Equality.lean
@@ -58,10 +58,6 @@ namespace Bind2Variant
   | arrow, arrow => true
   | allc, allc => true
   | arrowc, arrowc => true
-  | letopentype, letopentype => true
-  | letopen, letopen => true
-  | letctor, letctor => true
-  | insttype, insttype => true
   | _, _ => false
 end Bind2Variant
 
@@ -87,18 +83,14 @@ namespace Term
     beq x1 y1 && beq x2 y2 && beq x3 y3 && beq x4 y4
   | guard x1 x2 x3, guard y1 y2 y3 =>
     beq x1 y1 && beq x2 y2 && beq x3 y3
-  | letdata x1 x2, letdata y1 y2 => beq x1 y1 && beq x2 y2
   | letterm x1 x2 x3, letterm y1 y2 y3 =>
     beq x1 y1 && beq x2 y2 && beq x3 y3
-  | inst n1 x1 x2, inst n2 y1 y2 =>
-    n1 == n2 && beq x1 y1 && beq x2 y2
   | ctor1 v1 x1, ctor1 v2 x2 =>
     v1 == v2 && beq x1 x2
   | ctor2 v1 x1 x2, ctor2 v2 y1 y2 =>
     v1 == v2 && beq x1 y1 && beq x2 y2
   | bind2 v1 x1 x2, bind2 v2 y1 y2 =>
     v1 == v2 && beq x1 y1 && beq x2 y2
-  | decl x, decl y => beq x y
   | _, _ => false
 
   theorem eq_of_beq : Term.beq a b = true -> a = b := by
@@ -133,14 +125,9 @@ namespace Term
   case _ ih1 ih2 ih3 _ _ _ =>
     rw [ih1 h.1.1, ih2 h.1.2]
     rw [ih3 h.2]; simp
-  case _ ih1 ih2 _ _ =>
-    rw [ih1 h.1, ih2 h.2]; simp
   case _ ih1 ih2 ih3 _ _ _ =>
     rw [ih1 h.1.1, ih2 h.1.2]
     rw [ih3 h.2]; simp
-  case _ ih _ => rw [ih h]
-  case _ ih1 ih2 _ _ _ =>
-    rw [h.1.1, ih1 h.1.2, ih2 h.2]; simp
 
   theorem rfl : Term.beq a a = true := by
   induction a <;> simp at * <;> simp [*]
