SystemFD/Term/Substitution.lean
@@ -84,10 +84,7 @@ namespace Term
   | bind2 v t1 t2 => bind2 v (smap lf f t1) (smap lf (lf f) t2)
   | ite t1 t2 t3 t4 => ite (smap lf f t1) (smap lf f t2) (smap lf f t3) (smap lf f t4)
   | guard t1 t2 t3 => guard (smap lf f t1) (smap lf f t2) (smap lf f t3)
-  | letdata t1 t2 => letdata (smap lf f t1) (smap lf (lf f) t2)
   | letterm t1 t2 t3 => letterm (smap lf f t1) (smap lf f t2) (smap lf (lf f) t3)
-  | inst n t1 t2 => inst n (smap lf f t1) (smap lf (lf f) t2)
-  | decl t => decl (smap lf (lf f) t)
 end Term
 
 @[simp]
@@ -131,16 +128,8 @@ namespace Term
   theorem subst_bind2 : [σ]bind2 v t1 t2 = bind2 v ([σ]t1) ([^σ]t2) := by unfold Subst.apply; simp
 
   @[simp]
-  theorem subst_letdata: [σ]letdata t1 t2 = letdata ([σ]t1) ([^σ]t2) := by unfold Subst.apply; simp
-
-  @[simp]
   theorem subst_letterm: [σ]letterm t1 t2 t3 = letterm ([σ]t1) ([σ]t2) ([^σ]t3) := by unfold Subst.apply; simp
 
-  @[simp]
-  theorem subst_inst : [σ]inst n t1 t2 = inst n ([σ]t1) ([^σ]t2) := by unfold Subst.apply; simp
-
-  @[simp]
-  theorem subst_decl : [σ]decl t = decl ([^σ]t) := by unfold Subst.apply; simp
 
   theorem apply_id {t : Term} : [I]t = t := by
   have lem1 : ^I = @I Term := by
